$$
\left \{
\begin{array}{l}
\bar{u}_{\alpha}(\boldsymbol{x}) = u_{\alpha}(x_1,x_2) - x_3 w_{,\alpha} \\
\bar{u}_{3}(\boldsymbol{x}) = w(x_1,x_2)
\end{array}
\right .
,\quad \alpha = 1,2
$$
$$
\left \{
\begin{aligned}
\varepsilon_{\alpha \beta} &=\frac{1}{2}(u_{\alpha, \beta}+u_{\beta, \alpha})-x_{3}w_{, \alpha \beta} \\
\varepsilon_{\alpha 3} &=\frac{1}{2}\left(w_{, \alpha}-w_{,\alpha}\right) = 0 \\
\varepsilon_{33} &=0
\end{aligned}
\right .
$$
$$
\begin{align}
\begin{Bmatrix}
\sigma_{11} \\ \sigma_{22} \\ \sigma_{33} \\ \sigma_{12} \\ \sigma_{13} \\ \sigma_{23}
\end{Bmatrix} &= 
\frac{E}{(1+\nu)(1-2\nu)}
\begin{bmatrix}
1-\nu &   \nu &   \nu & 0 & 0 & 0 \\
  \nu & 1-\nu &   \nu & 0 & 0 & 0 \\
  \nu &   \nu & 1-\nu & 0 & 0 & 0 \\
    0 &     0 &     0 & \frac{(1-2\nu)}{2} & 0 & 0 \\
    0 &     0 &     0 & 0 & \frac{(1-2\nu)}{2} & 0 \\
    0 &     0 &     0 & 0 & 0 & \frac{(1-2\nu)}{2}
\end{bmatrix}
\begin{Bmatrix}
u_{1,1} - x_3 w_{,11} \\ u_{2,2} - x_3 w_{,22} \\ 0 \\ u_{1,2}+u_{2,1}-2x_3 w_{,12} \\ 0 \\ 0
\end{Bmatrix} \\ &=
\begin{Bmatrix}
u_{1,1} - x_3 w_{,11} \\ u_{2,2} - x_3 w_{,22} \\ 0 \\ u_{1,2}+u_{2,1}-2x_3 w_{,12} \\ 0 \\ 0
\end{Bmatrix}
\end{align}
$$
