The bar, beam and plate theory can be degenerated by [[❖ Elasticity|elasticity theory]]. The plate theory is concluded Kirchhoff-Love plate(thin plate) and Mindlin–Reissner plate(thick plate), since their one-dimensional theories are  Euler-Bernoulli beam and Timoshenko beam. The follow sections introduce these theories.
# Plate theory
## Mindlin-Reissner plate
Assuming that
$$
\left \{
\begin{array}{l}
\bar{u}_{\alpha}(\boldsymbol{x}) = u_{\alpha}(x_1,x_2) - x_3 \varphi_{\alpha} \\
\bar{u}_{3}(\boldsymbol{x}) = w(x_1,x_2)
\end{array}
\right .
,\quad \alpha = 1,2
$$
$$
\left \{
\begin{aligned}
\varepsilon_{\alpha \beta} &=\frac{1}{2}\left(u_{\alpha, \beta}+u_{\beta, \alpha}\right)-\frac{x_{3}}{2}\left(\varphi_{\alpha, \beta}+\varphi_{\beta, \alpha}\right) \\
\varepsilon_{\alpha 3} &=\frac{1}{2}\left(w_{, \alpha}-\varphi_{\alpha}\right) \\
\varepsilon_{33} &=0
\end{aligned}
\right .
$$
## Kirchhoff-Love plate
$$
\left \{
\begin{array}{l}
\bar{u}_{\alpha}(\boldsymbol{x}) = u_{\alpha}(x_1,x_2) - x_3 w_{,\alpha} \\
\bar{u}_{3}(\boldsymbol{x}) = w(x_1,x_2)
\end{array}
\right .
,\quad \alpha = 1,2
$$
$$
\left \{
\begin{aligned}
\varepsilon_{\alpha \beta} &=\frac{1}{2}(u_{\alpha, \beta}+u_{\beta, \alpha})-x_{3}w_{, \alpha \beta} \\
\varepsilon_{\alpha 3} &=\frac{1}{2}\left(w_{, \alpha}-w_{,\alpha}\right) = 0 \\
\varepsilon_{33} &=0
\end{aligned}
\right .
$$
## Timoshenko beam
$$
\left \{
\begin{array}{l}
\bar{u}_{1}(\boldsymbol{x}) = u(x_1) - x_3 \varphi(x_1) \\
\bar{u}_{2}(\boldsymbol{x}) = v(x_2) \\
\bar{u}_{3}(\boldsymbol{x}) = w(x_1,x_3)
\end{array}
\right .
$$
$$
\begin{Bmatrix}
\varepsilon_{11} \\ \varepsilon_{22} \\ \varepsilon_{33} \\ \varepsilon_{12} \\ \varepsilon_{13} \\ \varepsilon_{23} 
\end{Bmatrix} = 
\begin{Bmatrix}
u_{,1} - x_3 \varphi_{,1} \\ v_{,2} \\ w_{,3} \\ 0 \\ u_{3,1}-\varphi \\ 0 
\end{Bmatrix} = 
\begin{Bmatrix}
u_{,1} - x_3 \varphi_{,1} \\ \nu x_3 \varphi_{,1} \\ \nu x_3 \varphi_{,1} \\ 0 \\ u_{3,1}-\varphi \\ 0 
\end{Bmatrix}
$$
## Euler-Bernoulli beam
$$
\left \{
\begin{array}{l}
\bar{u}_{1}(\boldsymbol{x}) = u(x_1) - x_3 w_{,1} \\
\bar{u}_{2}(\boldsymbol{x}) = v(x_2) \\
\bar{u}_{3}(\boldsymbol{x}) = w(x_1,x_3)
\end{array}
\right .
$$
$$
\begin{Bmatrix}
\varepsilon_{11} \\ \varepsilon_{22} \\ \varepsilon_{33} \\ \varepsilon_{12} \\ \varepsilon_{13} \\ \varepsilon_{23} 
\end{Bmatrix} = 
\begin{Bmatrix}
u_{,1} - x_3 w_{,11} \\ v_{,2} \\ w_{,3} \\ 0 \\ w_{,1}-w_{,1} \\ 0 
\end{Bmatrix} = 
\begin{Bmatrix}
u_{,1} - x_3 w_{,11} \\ \nu x_3 w_{,11} \\ \nu x_3 w_{,11} \\ 0 \\ 0 \\ 0 
\end{Bmatrix}
$$
