# 弹塑性力学 作业

<center>Deadline: 2022年11月24日, 上课前交</center>

<center>作业采用电子版提交，电子版发送至群作业中</center>

1. A material is to be loaded to a stress state
    $$
    [\sigma_{ij}] = \begin{bmatrix}
        50 & -30 & 0 \\
        -30 & 90 & 0 \\
        0 & 0 & 0
    \end{bmatrix} \mathrm{MPa}
    $$
    
    Please show the minimum uniaxial yield stress $\sigma_Y$ of the material such that it does not fail, according to the
    (a) Tresca criterion  $f:=\tau_{\mathrm{max}}-\sigma_Y\le0$
    (b) Von-Mises criterion  $f:=\sqrt{2J_2}-\sigma_Y\le0$

    **Solution**:
    The principal stress of this stress state can be obtained as
    $$
    \sigma_1 = 106.05, \quad \sigma_2 = 33.94, \quad \sigma_3 = 0.0
    $$
    the $\tau_{\mathrm{max}}$ and $\sqrt{2J_2}$ are evaluated by
    $$
    \left \{
        \begin{split}
           &\tau_{\mathrm{max}} = \frac{1}{2}(\sigma_1-\sigma_3) = 106.05 \mathrm{MPa} \\
           &\sqrt{2J_2} = \sqrt{\frac{1}{3}((\sigma_1-\sigma_2)^2+(\sigma_2-\sigma_3)^2+(\sigma_3-\sigma_1)^2)} = 76.59 \mathrm{MPa}
        \end{split}
    \right .
    $$
    As the material does not fail with this stress state, the minimum yield stress can be given by
    $$
    \sigma_Y = 
    \left \{
        \begin{array}{l}
            106.06 \mathrm{MPa}, & \text{for Tresca criterion} \\
            76.59 \mathrm{MPa}, & \text{for Von-Mises criterion} 
        \end{array}
    \right .
    $$

2. Please state the following Tresca and Von-Mises criterion in 2D principal stress with plane stress assumption, and plot the yield surface with axes $(\sigma_1,\sigma_2)$. (Hint: the figure of $x^2-xy+y^2=1$ is shown in Fig.1)
    - Tresca criterion: $f:=\tau_{\mathrm{max}}-Y\le0$

    - Von-Mises criterion: $f:=\sqrt{2J_2}-\frac{1}{2}\sqrt{\frac{2}{3}}Y\le0$

    ![Fig.1](/Users/wujc/note/Excalidraw/20221110-2.png)

    **Solution**:
    For plane stress assumption of $\sigma_{3i}=0, \; i=1,2,3$, the $\tau_{\mathrm{max}}$ and $\sqrt{2J_2}$ can be written as
    $$
    \left \{
        \begin{split}
            \tau_{\mathrm{max}} &= \frac{1}{2}\max (|\sigma_1 - \sigma_2|, |\sigma_1|,|\sigma_2|) \\
            \sqrt{2J_2} &= \sqrt{\frac{2}{3}(\sigma_1^2+\sigma_1 \sigma_2+\sigma_2^2)} 
        \end{split}
    \right .
    $$
    the yield surface in terms of $(\sigma_1,\sigma_2)$ is listed as follow
    ![Fig.3](/Users/wujc/note/Excalidraw/20221115-4.png)

3. Given the yield stresses $\sigma_t$ and $\sigma_c$ in uniaxial tension and compression respectively, find the yield stress in shear, as shown in Fig.2, resulting from the following yield criterion: (a) Mohr-Coulomb, (b) Drucker-Prager.

    ![Fig.1](/Users/wujc/note/Excalidraw/20221110-1.png)

    **Solution**:
    For pure shear state, the principal stress is given by
    $$
    \sigma_1 = \sigma_s, \quad \sigma_2 = 0, \quad \sigma_3 = -\sigma_s
    $$
    (a) For Mohr-Coulomb criterion, the yield function can be expressed in terms of $\sigma_t$ and $\sigma_c$ as
    $$
    f:= \frac{1}{2}(\sigma_1-\sigma_3) - \frac{\sigma_c \sigma_t}{\sigma_c+\sigma_t} + \frac{1}{2}(\sigma_1+\sigma_3)\frac{\sigma_c-\sigma_t}{\sigma_c+\sigma_t} \le 0
    $$
    the yield stress in shear can be got by substituting principal stress of pure shear in yield function
    $$
    \frac{1}{2}(\sigma_1-\sigma_3) - \frac{\sigma_c \sigma_t}{\sigma_c+\sigma_t} + \frac{1}{2}(\sigma_1+\sigma_3)\frac{\sigma_c-\sigma_t}{\sigma_c+\sigma_t} = \sigma_s - \frac{\sigma_c \sigma_t}{\sigma_c+\sigma_t} = 0
    $$
    $$
    \sigma_s = \frac{\sigma_c \sigma_t}{\sigma_c+\sigma_t}
    $$

    (b) For Drucker-Prager criterion, the yield function can be expressed in terms of $\sigma_t$ and $\sigma_c$ as
    $$
    f:= \sqrt{2J_2} - \sqrt{\frac{1}{6}} \frac{\sigma_t \sigma_c}{\sigma_t+\sigma_c} - \sqrt{\frac{3}{2}}\frac{\sigma_t+\sigma_c}{\sigma_t-\sigma_c} I_1 \le 0
    $$
    substituting principal stress of pure shear leads to
    $$
    \sqrt{2J_2} - \sqrt{\frac{1}{6}} \frac{\sigma_t \sigma_c}{\sigma_t+\sigma_c} - \sqrt{\frac{3}{2}}\frac{\sigma_t+\sigma_c}{\sigma_t-\sigma_c} I_1 = \sqrt{2}\sigma_s - \sqrt{\frac{1}{6}} \frac{\sigma_t \sigma_c}{\sigma_t+\sigma_c} = 0
    $$
    $$
    \sigma_s = \frac{\sqrt{3}}{6} \frac{\sigma_t \sigma_c}{\sigma_t+\sigma_c}
    $$
